poly proof wip

examples/chacha20poly1305/src/chacha20poly1305.rs
@@ -14,29 +14,25 @@ pub fn init(key: ChaChaPolyKey, iv: ChaChaPolyIV) -> PolyState {
     poly1305_init(poly_key)
 }
 
-pub fn update_padded (m:&ByteSeq, st:PolyState) -> PolyState {
-    let mut st = st;
-    for i in 0..m.num_chunks(16) {
-        let (_, block) = m.get_chunk(16, i);
-        st = poly1305_update1(16,&block,st); // This is the only line that changes from poly1305_update.
-                                             // And then again it only makes a difference for poly1305_update_last
-    }
-    st
+pub fn poly1305_update_padded (m:&ByteSeq, st:PolyState) -> PolyState {
+    let st = poly1305_update_blocks(m,st);
+    let last = get_last_chunk(m,16);
+    poly1305_update_last(16,&last,st)
 }
 
 pub fn finish(aadlen:usize, cipherlen:usize, st:PolyState) -> Tag {
     let mut last_block = PolyBlock::new();
     last_block = last_block.update(0,&U64_to_le_bytes(U64(aadlen as u64)));
     last_block = last_block.update(8,&U64_to_le_bytes(U64(cipherlen as u64)));
-    let st = poly1305_update1(16,&SubBlock::from_seq(&last_block),st);
+    let st = poly1305_update_block(&last_block,st);
     poly1305_finish(st)
 }
 
 pub fn encrypt(key: ChaChaPolyKey, iv: ChaChaPolyIV, aad: &ByteSeq, msg: &ByteSeq) -> (ByteSeq, Tag) {
     let cipher_text = chacha20(key, iv, 1u32, msg);
     let mut poly_st = init(key,iv);
-    poly_st = update_padded(aad, poly_st);
-    poly_st = update_padded(&cipher_text, poly_st);
+    poly_st = poly1305_update_padded(aad, poly_st);
+    poly_st = poly1305_update_padded(&cipher_text, poly_st);
     let tag = finish(aad.len(),cipher_text.len(),poly_st);
     (cipher_text, tag)
 }
@@ -45,8 +41,8 @@ pub fn encrypt(key: ChaChaPolyKey, iv: ChaChaPolyIV, aad: &ByteSeq, msg: &ByteSe
 pub fn decrypt(key: ChaChaPolyKey, iv: ChaChaPolyIV, aad: &ByteSeq, cipher_text: &ByteSeq, tag: Tag) ->
        Option<ByteSeq> {
     let mut poly_st = init(key,iv);
-    poly_st = update_padded(aad, poly_st);
-    poly_st = update_padded(cipher_text, poly_st);
+    poly_st = poly1305_update_padded(aad, poly_st);
+    poly_st = poly1305_update_padded(cipher_text, poly_st);
     let my_tag = finish(aad.len(),cipher_text.len(),poly_st);
     if my_tag.declassify_eq(&tag) {
         Some(chacha20(key, iv, 1u32, cipher_text))
