examples/poly1305/src/poly1305.rs
@@ -19,6 +19,9 @@ bytes!(Tag, 16);
 // A byte sequence of length <= BLOCKSIZE
 pub type SubBlock = ByteSeq;
 
+// A length <= BLOCKSIZE
+pub type BlockIndex = usize;
+
 // This defines the field for modulo 2^130-5.
 // In particular `FieldElement` and `FieldCanvas` are defined.
 // The `FieldCanvas` is an integer type with 131-bit (to hold 2*(2^130-5)).
@@ -40,10 +43,18 @@ pub fn poly1305_encode_r (b:&PolyBlock) -> FieldElement {
     FieldElement::from_secret_literal(n)
 }
 
-pub fn poly1305_encode_block (len:usize, b:&SubBlock) -> FieldElement {
-    let n = U128_from_le_bytes(U128Word::from_slice(b,0,b.len())); // Silliness, from_seq should work but it panics
+pub fn poly1305_encode_block (b:&PolyBlock) -> FieldElement {
+    let n = U128_from_le_bytes(U128Word::from_seq(b));
     let f = FieldElement::from_secret_literal(n);
-    f + FieldElement::pow2(8 * len)
+    f + FieldElement::pow2(128)
+}
+
+// In Poly1305 as used in this spec, pad_len is always the length of b, i.e. there is no padding
+// In Chacha20Poly1305, pad_len is set to BLOCKSIZE
+pub fn poly1305_encode_last (pad_len:BlockIndex,b:&SubBlock) -> FieldElement {
+    let n = U128_from_le_bytes(U128Word::from_slice(b,0,b.len())); 
+    let f = FieldElement::from_secret_literal(n);
+    f + FieldElement::pow2(8 * pad_len)
 }
 
 pub fn poly1305_init (k:PolyKey) -> PolyState {
@@ -51,9 +62,45 @@ pub fn poly1305_init (k:PolyKey) -> PolyState {
     (FieldElement::ZERO(), r, k)
 }
 
-pub fn poly1305_update1 (len:usize, b:&SubBlock, st:PolyState) -> PolyState {
+pub fn poly1305_update_block (b:&PolyBlock, st:PolyState) -> PolyState {
     let (acc,r,k) = st;
-    ((poly1305_encode_block(len,b) + acc) * r,r,k)
+    ((poly1305_encode_block(b) + acc) * r,r,k)
+}
+
+pub fn get_full_chunk(m:&Seq<U8>,cs:usize,i:usize) -> Seq<U8> {
+    let (_len,block) = m.get_chunk(cs, i);
+    block
+}
+
+pub fn get_last_chunk(m:&Seq<U8>,cs:usize) -> Seq<U8> {
+    let nblocks = m.len() / cs;
+    let (_len,block) = m.get_chunk(cs, nblocks);
+    block
+}
+
+pub fn poly1305_update_blocks (m:&ByteSeq, st:PolyState) -> PolyState {
+    let mut st = st;
+    let nblocks = m.len() / BLOCKSIZE;
+    for i in 0..nblocks {
+        let block = PolyBlock::from_seq(&get_full_chunk(m,BLOCKSIZE, i));
+        st = poly1305_update_block(&block,st);
+    }
+    st
+}
+
+pub fn poly1305_update_last (pad_len:usize, b:&SubBlock, st:PolyState) -> PolyState {
+    let mut st = st;
+    if b.len() != 0 {
+        let (acc,r,k) = st;
+        st = ((poly1305_encode_last(pad_len,b) + acc) * r,r,k);
+    }
+    st
+}
+
+pub fn poly1305_update (m:&ByteSeq, st:PolyState) -> PolyState {
+    let st = poly1305_update_blocks(m,st);
+    let last = get_last_chunk(m,BLOCKSIZE);
+    poly1305_update_last(last.len(),&last,st)
 }
 
 pub fn poly1305_finish (st:PolyState) -> Tag {
@@ -64,17 +111,9 @@ pub fn poly1305_finish (st:PolyState) -> Tag {
     Tag::from_seq(&U128_to_le_bytes(a+n))
 }
 
-pub fn poly1305_update (m:&ByteSeq, st:PolyState) -> PolyState {
-    let mut st = st;
-    for i in 0..m.num_chunks(BLOCKSIZE) {
-        let (len, block) = m.get_chunk(BLOCKSIZE, i);
-        st = poly1305_update1(len,&block,st);
-    }
-    st
-}
-
 pub fn poly1305(m: &ByteSeq, key: PolyKey) -> Tag {
     let mut st = poly1305_init(key);
     st = poly1305_update(m,st);
     poly1305_finish(st)
 }
+
